renamed hypothesis in automated proof to avoid already introduced names. Plus removed direct reference to hypothesis

Tactic.v
@@ -9,12 +9,13 @@ From Ltac2 Require Import Message.
 From Ltac2 Require Import Control.
 From Ltac2 Require Import Std.
 
+(** TODO : rename variables to decrease the risk of them being already introduced *)
 
 Ltac2 rec introductions () :=
   (* introduces all variables and unfolds the definition *)
   match! goal with
   | [ h:_ |- ?g ] => match! g with
-                    | preserve_Injectivity ?f => unfold preserve_Injectivity; intros C v Hinj i j x y H
+                    | preserve_Injectivity ?f => unfold preserve_Injectivity; intros set_C view_v H_v_inj index_i index_j index_x index_y Hypthesis
                     | _ => intro; introductions ()
                     end
   | [ |- _ ] => intro; introductions ()
@@ -45,25 +46,20 @@ end).
 Ltac2 applyHinj (f:constr) :=
   (* use the injectivity hypothesis *)
    match! goal with
-  | [ h1 : Injective ?v, hx:(?t1 = (?x,?tx)), hy:(?t2 = (?y,?ty)), hi:(?t3 = (?i,?ti)), j:(?t4 = (?j,?tj)), h2 : _ |- _ ] => let h1' := Control.hyp h1 in let h2' := Control.hyp h2 in
-  assert (Heq : curry_totalApp (curry_partialApp &v (A := (&h::&C)) ($i,$ti)) ($f ($x,$tx)) =
-          curry_totalApp (curry_partialApp &v (A := (&h::&C)) ($j,$tj)) ($f ($y,$ty))
+  | [ h1 : Injective ?v, hx:(?t1 = (?x,?tx)), hy:(?t2 = (?y,?ty)), hi:(?t3 = (?i,?ti)), j:(?t4 = (?j,?tj)), h : nat, c : List nat, v : ViewArray _, h2 : _ |- _] => let h1' := Control.hyp h1 in let h2' := Control.hyp h2 in
+  let h := Control.hyp h in let c := Control.hyp c in
+  assert (Hypothesis_equality : curry_totalApp (curry_partialApp $v (A := ($h::$c)) ($i,$ti)) ($f ($x,$tx)) =
+          curry_totalApp (curry_partialApp $v (A := ($h::$c)) ($j,$tj)) ($f ($y,$ty))
         -> (($i,$ti),($f ($x,$tx))) = (($j,$tj),($f ($y,$ty))));
   try (apply injectivity_decomposition; apply $h1');
-  apply &Heq in $h2
+  apply &Hypothesis_equality in $h2
    | [ h1 : Injective ?v, hx:(?t1 = (?x,?tx)), hy:(?t2 = (?y,?ty)), h2 : _ |- _ ] => let h1' := Control.hyp h1 in let h2' := Control.hyp h2 in
   unfold Injective in *;
   apply $h1' with (x := $f ($x,$tx)) (y := $f ($y,$ty)) in $h2
 end.
 
 
-Ltac2 reordering_autoProof (f:constr) (fid:ident) (dim : int):=
-(* Semi-Automatic proof of correctness for reordering functions :
-  takes as inputs :
-  - a hint function, the reordering function, given as constr and ident
-  - the expected number of dimension (minus one) of the input viewArray
-  (cf. the examples in `Examples_automation.v`)
-*)
+Ltac2 reordering_autoProof1 (f:constr) (fid:ident) (dim : int):=
   introductions ();
   remember_destruction ();
   do dim (destruction ());
@@ -75,12 +71,48 @@ Ltac2 reordering_autoProof (f:constr) (fid:ident) (dim : int):=
   enter (fun () =>
     remember_destruction ();
     remember_destruction ();
-    subst2 ();
+    subst2 ()
+  ).
+
+
+Ltac2 reordering_autoProof2 (f:constr) (fid:ident) (dim : int):=
+  enter (fun () =>
     (applyHinj (f));
     let f' := VarRef (fid) in
-    unfold $f' in H;
-    inversion H;
+    unfold $f' in Hypthesis;
+    inversion Hypthesis;
     subst
   ).
+
+
+Ltac2 reordering_autoProof (f:constr) (fid:ident) (dim : int):=
+(* Semi-Automatic proof of correctness for reordering functions :
+  takes as inputs :
+  - a hint function, the reordering function, given as constr and ident
+  - the expected number of dimension (minus one) of the input viewArray
+  (cf. the examples in `Examples_automation.v`)
+  Note : it will only work with simple enough functions (when no case disjunction is needed)
+*)
+  reordering_autoProof1 f fid dim;
+  reordering_autoProof2 f fid dim.
+
+Definition selectProof {n : nat} {m : nat} {i : Idx n} (H : m > 0):
+  m*(to_nat i) < m*n.
+Proof.
+Admitted.
+
+Definition select {T : List nat} {n : nat} (m : nat) (H : m > 0) (v : ViewArray[[T;m*n]]) : ViewArray[[T;n]] :=
+  fun i => v (idx (m*n) (m*(to_nat i)) (selectProof H)).
+
+Proposition test : forall T n m (H : m > 0), preserve_Injectivity (select m H) (A := (m*n::T)).
+Proof.
+  intros T n m H'.
+  set (function := fun (x : Tuple (n::T)) => match x with | (i,tx) => (idx (m*n) (m*(to_nat i)) (selectProof H'),tx) end).
+  reordering_autoProof ('function) (@function) 0.
+  apply Nat.mul_cancel_l in H0. apply to_nat_injective in H0. subst. reflexivity ().
+  intro. subst. inversion H'.
+  apply Nat.mul_cancel_l in H2. apply to_nat_injective in H2. subst. reflexivity ().
+  intro. subst. inversion H'.
+Qed.
 
 
